example

compiler_test/beepl_test/BeePL_progs.v
@@ -7,7 +7,7 @@ BeePL_cond BeePL_app BeePL_funptr_ex1 BeePL_bpf_get_prandom BeePL_for_ex1 BeePL_
 BeePL_external_call BeePL_match_fail_ex1 BeePL_null_ptr BeePL_bitstring1 BeePL_globvar1
 BeePL_bpf_xdp_packet_count BeePL_bpf_xdp_packet_count1 BeePL_bpf_map_example1 BeePL_bpf_drop_xdp_packet_iPv6
 BeePL_bpf BeePL_bpf_handle_tp BeePL_add_ref BeePL_section BeePL_cast BeePL_cast1 BeePL_shift BeePL_bpf_map_null_check
-BeePL_bpf_safe_null_check BeePL_globvar_local beepl_success_load.BeePL_bpf_xdp1. 
+BeePL_bpf_safe_null_check BeePL_globvar_local beepl_success_load.BeePL_bpf_xdp1 beepl_success_load.BeePL_bpf_xdp2. 
 
 (* In this file you will see two definitions. One for example1 and the other for
    example1_atom_of_string. Those two definitions are extracted to OCaml by 
@@ -26,9 +26,9 @@ BeePL_bpf_safe_null_check BeePL_globvar_local beepl_success_load.BeePL_bpf_xdp1.
 
 (* Construct the BeePL.program *)
 
-Definition example1 : BeePL.program := @mkbprogram BeePL_bpf_xdp1.bcomposites 
-                                                   BeePL_bpf_xdp1.global_definitions 
-                                                   BeePL_bpf_xdp1.public_idents 
-                                                   BeePL_bpf_xdp1._main 
-                                                   BeePL_bpf_xdp1.bcomposite_correct
-                                                   BeePL_bpf_xdp1.ident_to_string.
+Definition example1 : BeePL.program := @mkbprogram BeePL_bpf_xdp2.bcomposites 
+                                                   BeePL_bpf_xdp2.global_definitions 
+                                                   BeePL_bpf_xdp2.public_idents 
+                                                   BeePL_bpf_xdp2._main 
+                                                   BeePL_bpf_xdp2.bcomposite_correct
+                                                   BeePL_bpf_xdp2.ident_to_string.
