compiler_test/beepl_test/beepl_success_load/BeePL_bpf_xdp2.v
@@ -1,0 +1,84 @@
+Require Import Integers AST Ctypes BeePL BeeTypes BeePL_values BeePL_typechecker BeePL_notations BeePL_bpf. 
+From Coq Require Import String ZArith.
+From compcert Require Import Csyntaxdefs.
+Import Csyntaxdefs.CsyntaxNotations.
+Local Open Scope list_scope.
+Local Open Scope string_scope.
+Local Open Scope csyntax_scope.
+
+(*#include <linux/bpf.h>
+#include <bpf/bpf_helpers.h>
+
+SEC("xdp")
+int xdp_prog(struct xdp_md *ctx) {
+    bpf_printk("Hello");
+    return XDP_PASS;
+}
+
+char _license[] SEC("license") = "Dual BSD/GPL"; *)
+
+
+Definition dattr := {| attr_volatile := false; attr_alignas := None |}.
+Definition _ctx : ident := $"ctx".
+Definition _r : ident := $"r".
+Definition ___stringlit_1 : ident := $"__stringlit_1".
+Definition _xdp_packet_count : ident := $"xdp_packet_count".
+Definition _main : ident := $"main".
+
+Definition ident_to_string : list (ident * string) := ident_to_string_hf ++ ident_to_string_xdp_md ++
+                                                      ((_ctx, "ctx") :: (___stringlit_1, "__stringlit_1") ::
+                                                       (_r, "r") ::
+                                                       (_xdp_packet_count, "xdp_packet_count") :: 
+                                                       (_main, "main") :: nil).
+
+Definition v___stringlit_1 := {|
+  gvar_info := (tbarray tint8s 6 noattr);
+  gvar_init := (Init_int8 (Int.repr 72) :: Init_int8 (Int.repr 101) ::
+                Init_int8 (Int.repr 108) :: Init_int8 (Int.repr 108) ::
+                Init_int8 (Int.repr 111) :: Init_int8 (Int.repr 0) :: nil);
+  gvar_readonly := true;
+  gvar_volatile := false
+|}.
+
+Definition f_xdp_packet_count : BeePL.function := {| 
+                                   fn_return := tint32s;
+                                   fn_effect := (Io :: nil);
+                                   fn_callconv := cc_default;
+                                   fn_args := (_ctx, tpstruct _xdp_md) :: nil ;
+                                   fn_vars := (_r, tint32s) :: nil;
+                                   fn_body := Bind _r tint32s 
+                                                (App (Var bpf_printk (tfun (trint8s :: nil) (Io :: nil) tint32s))
+                                                                  (Var ___stringlit_1 (tbarray tint8s 6 noattr) :: nil) tint32s)
+                                                (cint (Int.repr 2) tint32s) tint32s;
+                                   is_ebpf := true |}.
+
+Definition bcomposites : list bcomposite_definition := bcomposites_xdp_md.
+
+Definition global_definitions : list (ident * AST.globdef BeePL.fundef BeeTypes.type * option string) 
+   :=  (___stringlit_1, Gvar v___stringlit_1, None) ::
+       (bpf_printk, AST.Gfun(BeePL.External bpf_printk_ef
+                                     (trint8s :: nil) tint32s
+                                     {|cc_vararg:=(Some (Z.of_nat 1)); cc_unproto:=false; cc_structret:=false|}), None) ::
+       (_xdp_packet_count, AST.Gfun(BeePL.Internal (f_xdp_packet_count)), Some "xdp") :: nil.
+
+Definition public_idents : list ident := (_xdp_packet_count :: nil).
+
+Lemma bcomposite_correct :
+  wf_bcomposites bcomposites.
+Proof.
+  unfold wf_bcomposites.
+  unfold build_bcomposite_env; simpl; constructor. 
+Qed.
+
+(*Definition example1 : BeePL.program := @mkbprogram bcomposites 
+                                                   global_definitions 
+                                                   public_idents 
+                                                   _xdp_packet_count 
+                                                   bcomposite_correct
+                                                   ident_to_string.
+
+Compute (type_check_expr example1.(prog_comp_env) 
+                         (bind_vars (bind_vars empty_context f_xdp_packet_count.(fn_args)) f_xdp_packet_count.(fn_vars)) empty_context f_xdp_packet_count.(fn_body)).
+
+
+Compute (type_check_program example1). *) (* Type checks! *)
